Properly handle ghost-witness

Source/Dafny/Compiler-cpp.cs
@@ -997,7 +997,7 @@ namespace Microsoft.Dafny {
         }
       } else if (cl is SubsetTypeDecl) {
         var td = (SubsetTypeDecl)cl;
-        if (td.Witness != null) {
+        if (td.WitnessKind == SubsetTypeDecl.WKind.Compiled) {
           return td.Module.CompileName + "::class_" + td.CompileName + "::Witness";
         } else if (td.WitnessKind == SubsetTypeDecl.WKind.Special) {
           // WKind.Special is only used with -->, ->, and non-null types:
