Source/Dafny/Compiler-java.cs
@@ -3008,7 +3008,7 @@ namespace Microsoft.Dafny{
         }
       } else if (cl is SubsetTypeDecl) {
         var td = (SubsetTypeDecl)cl;
-        if (td.Witness != null) {
+        if (td.WitnessKind == SubsetTypeDecl.WKind.Compiled) {
           return FullTypeName(udt) + ".defaultValue()";
         } else if (td.WitnessKind == SubsetTypeDecl.WKind.Special) {
           // WKind.Special is only used with -->, ->, and non-null types:
